Demo/Driver.v
@@ -5,6 +5,8 @@ Require Import Printing.
 Require Import Generation.
 Require Import Indist.
 
+Require Import String.
+Local Open Scope string.
 Definition SSNI (t : table) (v : @Variation State) : Property :=
   let '(V st1 st2) := v in
   let '(St _ _ _ (_@l1)) := st1 in
@@ -14,23 +16,38 @@ Definition SSNI (t : table) (v : @Variation State) : Property :=
       | L,L  => 
         match exec t st1, exec t st2 with
           | Some st1', Some st2' => property (indist st1' st2')
-          | _, _ => property rejected 
+          | _, _ => collect "L,L,FAIL" true (* property rejected *)
+        end
+      | H, H => 
+        match exec t st1, exec t st2 with
+          | Some st1', Some st2' =>
+            if is_atom_low (st_pc st1') && is_atom_low (st_pc st2') then
+              property (indist st1' st2') 
+            else if is_atom_low (st_pc st1') then
+              property (indist st2 st2') 
+            else 
+              property (indist st1 st1')
+          | _, _ => property rejected
         end
       | H,_ => 
         match exec t st1 with
           | Some st1' => property (indist st1 st1')
-          | _ => property rejected
+          | _ => collect "H,_,FAIL" true (* property rejected*)
         end
       | _,H => 
         match exec t st2 with
           | Some st2' => property (indist st2 st2')
-          | _ => property rejected
+          | _ => collect "L,H,FAIL" true (* property rejected *)
         end
     end
-  else property rejected.
+  else collect "Not indist!" true (* property rejected *) .
 
 Definition prop_SSNI := 
   forAllShrink show gen_variation_state (fun _ => nil) (SSNI default_table).
+
+Definition prop_gen_indist := 
+  forAllShrink show gen_variation_state (fun _ => nil) 
+               (fun v => let '(V st1 st2) := v in indist st1 st2).
 
 Definition main := 
   showResult (quickCheck prop_SSNI).
