Demo/Indist.v
@@ -1,3 +1,4 @@
+Require Import QuickChick.
 Require Import ZArith.
 Require Import List.
 
@@ -60,6 +61,14 @@ Instance indist_state : Indist State :=
   indist st1 st2 :=
     let '(St imem1 mem1 stk1 pc1) := st1 in
     let '(St imem2 mem2 stk2 pc2) := st2 in
-    indist mem1 mem2 && indist stk1 stk2 && indist pc1 pc2
+    if negb (indist mem1 mem2) then trace "Memory" false
+    else if negb (indist pc1 pc2) then trace "PC" false
+    else let (stk1',stk2') := 
+           match pc1 with 
+             | _ @ H => (cropTop stk1, cropTop stk2)
+             | _ => (stk1, stk2)
+           end in
+    if negb (indist stk1' stk2') then trace "Stack" false
+    else true
 |}.
 
